rocq-osiris/theories/program_logic/rules/array_rules.v
@@ -4,23 +4,26 @@ From osiris.program_logic Require Import ewp.
 From osiris.program_logic.rules Require Import impure_rules stop_rules.
 From osiris.logic Require Import list_z.
 
+Definition array : Type := list loc.
+
+Global Instance : Encode array := { encode arr := VArray arr }.
+Global Instance : Observe array (list loc) := { observe a := a }.
+
 Section array_resources.
 
   Context `{!osirisGS Σ}.
 
-  Definition isArray (a : val) (n : Z) : iProp Σ :=
-    ∃ (ls : list loc),
-      ⌜a = VArray ls⌝ ∗
-      ⌜length ls = n⌝ ∗
-      ⌜0 ≤ n < max_array⌝.
+  Definition isArray (a : array) (n : Z) : iProp Σ :=
+      ⌜length a = n⌝ ∗ ⌜0 ≤ n ≤ max_array⌝.
 
   Global Instance is_array_persistent a n : Persistent (isArray a n).
   Proof. apply _. Qed.
 
-  Definition isSlice `{Encode A} dq (a : val) (i : Z) (xs : list A) : iProp Σ :=
-    ∃ (ls : list loc),
-      ⌜a = VArray ls⌝ ∗ ⌜0 ≤ i ∧ i + length xs ≤ length ls⌝ ∗
-      [∗ list] l;x ∈ take (length xs) (drop i ls); xs, pointsto l dq (V #x).
+  Definition isSlice `{Encode A} dq (ls : array) (i : Z) (xs : list A) : iProp Σ :=
+    ⌜0 ≤ i ∧ i + length xs ≤ length ls⌝ ∗
+    [∗ list] l;x ∈ take (length xs) (drop i ls); xs, pointsto l dq (V #x).
+
+  Arguments isSlice {_ _} dq a i xs : rename.
 
   Lemma leq_length {A} (i : Z) (l : list A) :
     0 ≤ i ≤ length l →
@@ -79,7 +82,7 @@ Section array_resources.
    Proof.
      intros -> ->.
      iStartProof; iSplit; iIntros "Hslice".
-     - iDestruct "Hslice" as "(%ls & -> & [%Hpos %Hlen] & Hslice)".
+     - iDestruct "Hslice" as "([%Hpos %Hlen] & Hslice)".
        rewrite length_app in Hlen.
        replace (i + (length ys + length zs))
          with (i + length ys + length zs) in Hlen by lia.
@@ -87,37 +90,38 @@ Section array_resources.
        assert (0 ≤ length ys)%Z by apply (length_nonneg).
        assert (0 ≤ length zs)%Z by apply (length_nonneg).
        assert (0 ≤ i ∧ 0 ≤ length ys ∧ 0 ≤ length zs) as Hpos' by lia.
-       destruct (decompose_list _ _ _ ls Hpos' Hlen)
+       destruct (decompose_list _ _ _ a Hpos' Hlen)
          as (li & lys & lzs & lextra & -> & Hlen1 & Hlen2 & Hlen3).
+       rewrite /sub /seg.
        drop. take.
        iPoseProof (big_sepL2_app_inv with "Hslice") as "[Hslice1 Hslice2]".
        { rewrite /length in Hlen2. lia. }
        iSplitL "Hslice1".
-       + iExists _. iSplit; first done. iSplit.
+       + iSplit.
          { iPureIntro. rewrite !length_app in Hlen |-*. lia. }
+         rewrite /sub /seg.
          drop. take.
          iApply "Hslice1".
-       + iExists _. iSplit; first done. iSplit.
+       + iSplit.
          { iPureIntro. rewrite !length_app in Hlen |- *. lia. }
+         rewrite /sub /seg.
          drop. take.
          iApply "Hslice2".
      - iDestruct "Hslice" as "(Hslice1 & Hslice2)".
-       iDestruct "Hslice1" as "(%ls & %Harr & [%Hpos %Hlen] & Hslice1)".
-       iDestruct "Hslice2" as "(%ls' & %Harr' & [%Hpos' %Hlen'] & Hslice2)".
-       rewrite Harr' in Harr; inversion Harr; subst.
-       iExists ls. iSplit; first done. iSplit.
+       iDestruct "Hslice1" as "([%Hpos %Hlen] & Hslice1)".
+       iDestruct "Hslice2" as "([%Hpos' %Hlen'] & Hslice2)".
+       iSplit.
        { iPureIntro. rewrite length_app. lia. }
        (* Decompose [ls] into [li ++ lys ++ lzs ++ lextra]. *)
-       assert (0 ≤ length ys) by apply length_nonneg.
-       assert (0 ≤ length zs) by apply length_nonneg.
+       length_nonneg ys. length_nonneg zs.
        assert (0 ≤ i ∧ 0 ≤ length ys ∧ 0 ≤ length zs) as Hpos'' by lia.
-       destruct (decompose_list _ _ _ ls Hpos'' Hlen')
+       destruct (decompose_list _ _ _ a Hpos'' Hlen')
          as (li & lys & lzs & lextra & -> & Hlen1 & Hlen2 & Hlen3).
        drop. take.
        iApply (big_sepL2_app with "Hslice1 Hslice2").
    Qed.
 
-   Definition isArrayCell `{Encode A} dq (a : val) (i : nat) (x : A) : iProp Σ :=
+   Definition isArrayCell `{Encode A} dq (a : array) (i : nat) (x : A) : iProp Σ :=
      isSlice dq a i [x].
 
  End array_resources.
@@ -128,19 +132,23 @@ Section array_resources.
 
    Context {η : env} {E : coPset} {Ψ : iEff Σ}.
 
+   Lemma imp_as_array {ζ} (m : microvx) (Φ : array → iProp Σ) :
+     imp m @ E <|Ψ|> ⟨⟨ ζ ⟩⟩ {{ Φ }} -∗
+     imp as_array m @ E <|Ψ|> ⟨⟨ ζ ⟩⟩ {{ Φ }}.
+   Proof.
+     iIntros "Hm".
+     iApply (imp_bind with "Hm").
+     iIntros (a) "HΦ".
+     iApply (imp_ret with "HΦ"); encode.
+   Qed.
+
    Lemma imp_EArrayLength {ζ} (n : Z) e :
      imp eval η e @ E <|Ψ|> ⟨⟨ ζ ⟩⟩ {{ λ a, isArray a n }} -∗
      imp eval η (EArrayLength e) @ E <|Ψ|> ⟨⟨ ζ ⟩⟩ {{ λ n', ⌜n' = n⌝ }}.
    Proof.
      iIntros "He". simpl_eval.
      iApply (imp_bind _ _ (λ ls, ret (VInt (repr (length ls)))) with "[He]").
-     { rewrite /as_array.
-       iApply (imp_bind _ _ (λ v, val_as_array v) with "He").
-       iIntros (a) "#Harray".
-       iDestruct "Harray" as "(%ls & -> & Harray)". simpl.
-       iApply (imp_ret ls ls).
-       instantiate (1 := Build_Observe (list loc) _ (list loc) id). reflexivity.
-       iExact "Harray". }
+     { iApply (imp_as_array with "He"). }
      iIntros (ls) "(%Hlen & %Hbound)".
      change (♯ls) with ls.
      iApply (imp_ret (VInt (repr (length ls))) (length ls)%Z). encode.
@@ -148,17 +156,17 @@ Section array_resources.
    Qed.
 
    Lemma array_size_representable i :
-     0 ≤ i < max_array →
+     0 ≤ i ≤ max_array →
      representable i.
    Proof.
-     intros (Hpos & Hlt).
+     intros (Hpos & Hle).
      constructor.
      - rewrite min_signed_eq.
        transitivity 0; last assumption.
        apply Z.opp_nonpos_nonneg. apply Z.lt_le_incl, Z.gt_lt.
        apply Coqlib.two_power_nat_pos.
-     - pose proof (h := (Z.lt_trans i max_array max_signed Hlt max_array_length)).
-       apply Z.lt_le_incl, h.
+     - transitivity (max_array); auto.
+       apply Z.lt_le_incl, max_array_length.
    Qed.
 
    Lemma list_elem_of_split_length {A : Type} (l : list A) (i : Z) (x : A) :
@@ -192,52 +200,47 @@ Section array_resources.
    Qed.
 
    Lemma imp_EArrayMake `{Encode A} {ζ} {e1 e2} (n : Z) (Φ : A → iProp Σ) :
-     ⌜0 ≤ n < max_array⌝ -∗
+     ⌜0 ≤ n ≤ max_array⌝ -∗
      imp eval η e1 @ E <|Ψ|> ⟨⟨ ζ ⟩⟩ {{ λ i, ⌜i = n⌝ }} -∗
      imp eval η e2 @ E <|Ψ|> ⟨⟨ ζ ⟩⟩ {{ Φ }} -∗
      imp eval η (EArrayMake e1 e2) @ E <|Ψ|> ⟨⟨ ζ ⟩⟩
-       {{ λ a, ∃ x, Φ x ∗ isArray a n ∗ isSlice (DfracOwn 1) a 0 (replicate n x) }}.
+       {{ λ (a : array), ∃ x, Φ x ∗ isArray a n ∗ isSlice (DfracOwn 1) a 0 (replicate n x) }}.
    Proof.
      iIntros (Hbound) "He1 He2". simpl_eval.
-     iApply (@imp_Par _ _ val val exn _ _
-               _ _ _ _ _ _ _ _ _ _ _ _ _
+     iApply (imp_Par
                _ _ _ _ (as_int (eval η e1)) _ (pfbind inject2
                (λ '(n0, v),
-                  if ((0 <=? signed n0) && (signed n0 <? max_array))%bool
+                  if ((0 <=? signed n0) && (signed n0 <=? max_array))%bool
                   then
                    Stop CAllocn (replicate (signed n0) v)
                      (pfbind inject2 (λ ls : list loc, ret (VArray ls)))
                   else crash "invalid_argument: Array.make")) with "[He1] He2").
-     { rewrite /as_int.
-       iApply (imp_bind _ _ (λ v, val_as_int v) with "He1").
-       iIntros (?) "-> /=".
-       iApply (imp_ret (repr n) n). instantiate (1 := Build_Observe Z _ int repr). reflexivity.
-       instantiate (1 := (λ i, ⌜i = n⌝)%I). done. }
+     { iApply (imp_as_int with "He1"). }
+     rewrite /continue /discontinue /=.
      iSplit; last iSplit.
      - iIntros (e) "Hζ !>".
-       iApply (imp_throw with "Hζ").
+       iApply (@imp_throw _ _ array val with "Hζ").
      - iIntros (e) "Hζ !>".
-       iApply (imp_throw with "Hζ").
-     - iIntros (? a) "-> Hφ !>".
-       rewrite /continue /=.
+       iApply (@imp_throw _ _ array val with "Hζ").
+     - iIntros (? a) "-> Hφ !> /=".
        rewrite bind_ret.
        rewrite signed_repr; last apply array_size_representable, Hbound.
        assert (0 <=? n = true) as -> by lia.
-       assert (n <? max_array = true) as -> by lia.
-       iApply imp_allocn.
+       assert (n <=? max_array = true) as -> by lia.
+       simpl.
+       iApply (imp_allocn _ (pfbind inject2 (λ ls : list loc, ret (VArray ls)))).
        iIntros "!>" (ls) "Hpts".
        iPoseProof (big_sepL2_length with "Hpts") as "%Hlen'".
        assert (length ls = n) as Hlen.
        { pose proof (length_replicate n #a) as Hlen_z.
          rewrite /length in Hlen_z |- *. lia. }
        rewrite /continue /=.
-       iApply imp_ret. encode.
+       iApply (imp_ret (VArray ls) ls). encode.
        iFrame.
        iSplitR.
-       { iExists ls; auto. }
-       iExists ls. iSplit; first done.
-       rewrite length_replicate.
-       iSplit; first (iPureIntro; lia).
+       { iPureIntro. auto. }
+       iSplit.
+       { iPureIntro; rewrite length_replicate. lia. }
        drop. take.
        iApply big_sepL2_alt.
        iSplit; first iPureIntro.
@@ -260,15 +263,15 @@ Section array_resources.
          iPureIntro. lia.
    Qed.
 
-   Lemma imp_EArrayUnsafeGet2 `{Encode A, Inhabited A} {Φ : A → iProp Σ} {ζ} (Φ1 : val → iProp Σ) (Φ2 : Z → iProp Σ) e1 e2 :
-     imp eval η e1 @ E <|Ψ|> ⟨⟨ ζ ⟩⟩ {{ λ a, ∃ n, isArray a n ∗ Φ1 a }} -∗
+   Lemma imp_EArrayGet2 `{Encode A, Inhabited A} {Φ : A → iProp Σ} {ζ} (Φ1 : array → iProp Σ) (Φ2 : Z → iProp Σ) e1 e2 :
+     imp eval η e1 @ E <|Ψ|> ⟨⟨ ζ ⟩⟩ {{ λ a, Φ1 a }} -∗
      imp eval η e2 @ E <|Ψ|> ⟨⟨ ζ ⟩⟩ {{ λ i, Φ2 i }} -∗
      (∀ a i, Φ1 a -∗ Φ2 i -∗
              ∃ n, isArray a n ∗
              ∃ dq j xs (x : A),
                ▷ (⌜j ≤ i⌝ ∗ ⌜i - j < length xs⌝ ∗ isSlice dq a j xs ∗ ⌜xs !!! (i - j) = x⌝) ∗
                ▷ (isSlice dq a j xs -∗ Φ x)) -∗
-     imp eval η (EArrayUnsafeGet e1 e2) @ E <|Ψ|> ⟨⟨ ζ ⟩⟩ {{ Φ }}.
+     imp eval η (EArrayGet e1 e2) @ E <|Ψ|> ⟨⟨ ζ ⟩⟩ {{ Φ }}.
    Proof.
      iIntros "He1 He2 P". simpl_eval.
      iApply (imp_Par _ _ _ _ _ _ (pfbind inject2
@@ -277,23 +280,13 @@ Section array_resources.
                   | Some l => load l
                   | None => crash "index out of bounds"
                   end)) with "[He1] [He2]").
-     { rewrite /as_array.
-       iApply (imp_bind _ _ (λ v, val_as_array v) with "He1").
-       iIntros (a) "(%n & (%ls & -> & Harr) & HΦ1)".
-       iApply (imp_ret ls ls).
-       instantiate (1 := Build_Observe (list loc) _ (list loc) id). reflexivity.
-       instantiate (1 := (λ ls', Φ1 (VArray ls'))%I). done. }
-     { rewrite /as_int.
-       iApply (imp_bind _ _ (λ v, val_as_int v) with "He2").
-       iIntros (i) "HΦ2".
-       iApply (imp_ret (repr i) i).
-       instantiate (1 := Build_Observe (Z) _ (int) repr). reflexivity.
-       iExact "HΦ2". }
+     { iApply (imp_as_array with "He1"). }
+     { iApply (imp_as_int with "He2"). }
      iSplit; last iSplit.
      { iIntros (e) "Hζ !>".
-       iApply (imp_throw with "Hζ"). }
+       iApply (@imp_throw _ _ A val with "Hζ"). }
      { iIntros (e) "Hζ !>".
-       iApply (imp_throw with "Hζ"). }
+       iApply (@imp_throw _ _ A val with "Hζ"). }
      iIntros (ls i) "HΦ1 HΦ2".
      iDestruct ("P" with "HΦ1 HΦ2")
        as "(%n & #Harr & %dq & %j & %xs & %x & P)".
@@ -301,10 +294,8 @@ Section array_resources.
      iNext.
      iDestruct "P" as "((%Hle & %Hlt & Hslice & %Htotal_lookup) & P)".
 
-     iDestruct "Harr" as "(% & %Heq & %Hlen' & %Hbound)".
-     iDestruct "Hslice" as "(% & %Heq' & %Hlen & Hslice)".
-     inversion Heq; subst ls0; clear Heq.
-     inversion Heq'; subst ls1; clear Heq'.
+     iDestruct "Harr" as "(%Hlen' & %Hbound)".
+     iDestruct "Hslice" as "(%Hlen & Hslice)".
 
      (* Decompose [ls] into [lj ++ slice ++ _]. *)
      pose proof (cut_out_slice j (length xs) ls ltac:(lia) ltac:(lia))
@@ -343,13 +334,14 @@ Section array_resources.
      rewrite <- app_comm_cons.
      rewrite lookup_cons_eq_0.
 
-     iApply (imp_load with "Hl").
+     iApply (@imp_load _ _ val exn A with "Hl").
      rewrite /continue; iIntros "!> Hl /=".
-     iApply imp_ret. encode. rewrite Htotal_lookup. iApply "P".
+     iApply (@imp_ret _ _ A val); first encode.
+     rewrite Htotal_lookup. iApply "P".
      iCombine ("Hl Hslice2") as "Hslice2".
      iPoseProof (big_sepL2_cons (λ _ l' x', pointsto l' dq (V #x')) with "Hslice2") as "Hslice2".
      iPoseProof (big_sepL2_app with "Hslice1 Hslice2") as "Hslice".
-     iExists ls. iSplit; first auto. iSplit.
+     iSplit.
      { iPureIntro. lia. }
      rewrite {1}Hls.
      rewrite Hj. rewrite drop_app drop_all Z.sub_diag drop_none. simpl.
@@ -359,19 +351,19 @@ Section array_resources.
      iApply "Hslice".
    Qed.
 
-   Lemma imp_EArrayUnsafeGet `{Encode A, Inhabited A} {ζ} a (k n : Z) (i j : Z) dq (xs : list A) x e1 e2 :
+   Lemma imp_EArrayGet `{Encode A, Inhabited A} {ζ} a (k n : Z) (i j : Z) dq (xs : list A) x e1 e2 :
      ⌜j ≤ i⌝ -∗
      ⌜i - j < length xs⌝ -∗
-     ⌜xs !!! (i - j)%Z = x⌝ -∗
+     ⌜xs !!! (i - j) = x⌝ -∗
      isArray a n -∗
      ▷ isSlice dq a j xs -∗
      imp eval η e1 @ E <|Ψ|> ⟨⟨ ζ ⟩⟩ {{ λ a', ⌜a' = a⌝ }} -∗
      imp eval η e2 @ E <|Ψ|> ⟨⟨ ζ ⟩⟩ {{ λ i', ⌜i' = i⌝ }} -∗
-     imp eval η (EArrayUnsafeGet e1 e2) @ E <|Ψ|> ⟨⟨ ζ ⟩⟩
+     imp eval η (EArrayGet e1 e2) @ E <|Ψ|> ⟨⟨ ζ ⟩⟩
            {{ λ v, ⌜v = x⌝ ∗ isSlice dq a j xs }}.
    Proof.
      iIntros (Hi Hlookup Hlen) "#Harr Hslice He1 He2".
-     iApply (imp_EArrayUnsafeGet2 with "[He1] He2").
+     iApply (imp_EArrayGet2 with "[He1] He2").
      { iApply (imp_mono_ret with "He1").
        iIntros (?) "->". iFrame "#".
        instantiate (1 := (λ a', ⌜a' = a⌝)%I). done. }
@@ -380,103 +372,5 @@ Section array_resources.
      iFrame "%". iFrame.
      iIntros "!> $". done.
    Qed.
-
-   Lemma imp_EArrayGet `{Encode A, Inhabited A} {ζ} a (k n : Z) (i j : Z) dq (xs : list A) x e1 e2 :
-     ⌜j ≤ i⌝ -∗
-     ⌜i - j < length xs⌝ -∗
-     ⌜xs !!! (i - j)%Z = x⌝ -∗
-     isArray a n -∗
-     ▷ isSlice dq a j xs -∗
-     imp eval η e1 @ E <|Ψ|> ⟨⟨ ζ ⟩⟩ {{ λ a', ⌜a' = a⌝ }} -∗
-     imp eval η e2 @ E <|Ψ|> ⟨⟨ ζ ⟩⟩ {{ λ i', ⌜i' = i⌝ }} -∗
-     imp eval η (EArrayGet e1 e2) @ E <|Ψ|> ⟨⟨ ζ ⟩⟩
-       {{ λ v, ⌜v = x⌝ ∗ isSlice dq a j xs }}.
-   Proof.
-     iIntros (Hi Hlen' Hlookup) "#Harr Hslice He1 He2".
-     iDestruct "Harr" as "(% & -> & %Hlen & %Hbound)".
-     simpl_eval.
-     iApply (imp_Par _ _ _ _ _ _ (pfbind inject2
-               (λ '((ls0, i0) : list loc * int),
-                  match ls0 !! signed i0 with
-                  | Some l => load l
-                  | None => crash "invalid_argument: index out of bounds"
-                  end)) with "[He1] [He2]").
-     { rewrite /as_array.
-       iApply (imp_bind _ _ (λ v, val_as_array v) with "He1").
-       iIntros (?) "->".
-       iApply (imp_ret ls ls).
-       instantiate (1 := Build_Observe (list loc) _ (list loc) id). reflexivity.
-       instantiate (1 := (λ ls', ⌜ls' = ls⌝)%I). done. }
-     { rewrite /as_int.
-       iApply (imp_bind _ _ (λ v, val_as_int v) with "He2").
-       iIntros (?) "->".
-       iApply (imp_ret (repr i) i).
-       instantiate (1 := Build_Observe (Z) _ (int) repr). reflexivity.
-       instantiate (1 := (λ i', ⌜i' = i⌝)%I). done. }
-     iSplit; last iSplit.
-     { iIntros (e) "Hζ !>".
-       iApply (imp_throw with "Hζ"). }
-     { iIntros (e) "Hζ !>".
-       iApply (imp_throw with "Hζ"). }
-     iIntros (? ?) "-> ->".
-     rewrite /continue /= bind_ret.
-     iNext.
-
-     iDestruct "Hslice" as "(% & %Heq' & %Hlen'' & Hslice)".
-     inversion Heq'; subst ls0; clear Heq'.
-
-     (* Decompose [ls] into [lj ++ slice ++ _]. *)
-     pose proof (cut_out_slice j (length xs) ls ltac:(lia) ltac:(lia))
-       as (lj & slice & lextra & Hls & Hj & Hslice).
-     (* Turn [take _ (drop _ ls)] into [slice]. *)
-     rewrite Hj {1}Hls. drop.
-     rewrite Hslice. take.
-
-     assert (¬ (i - j < 0)) as Heqf by lia.
-
-     rewrite (signed_repr i); last (apply array_size_representable; lia).
-     assert (list_z.valid (i - j) xs) as Hvalid by lia.
-     pose proof (list_lookup_lookup_total_valid xs (i - j) Hvalid) as Hlookup'.
-
-     (* [Decompose [xs] intl [xk ++ x :: _]. *)
-     pose proof (list_elem_of_split_length xs (i - j) _ Hlookup')
-       as (xk & xrest & Hxs & Hxk).
-     rewrite {1}Hxs.
-
-     (* Inversions on [Hslice] gives us that
-        [slice] = [slicek ++ l :: _]. *)
-     iDestruct (big_sepL2_app_inv_r with "Hslice")
-       as "(%slicek & %slice' & -> & Hslice1 & Hslice2)".
-     iDestruct (big_sepL2_cons_inv_r with "Hslice2") as
-       "(%l & %slicerest & -> & Hl & Hslice2)".
-
-     (* We can now prove that [ls !! i] = [Some l]. *)
-     rewrite Hls lookup_app_r; last lia.
-     rewrite <- Hj.
-     rewrite <- app_assoc. iPoseProof (big_sepL2_length with "Hslice1") as "%Hleneq".
-     assert (length ls = j + length slicek + 1 + length slicerest + length lextra).
-     { rewrite Hls. rewrite !length_app. rewrite length_cons. lia. }
-     assert (length slicek = length xk) by (rewrite /length; lia).
-     rewrite lookup_app_r; last lia.
-     assert (i - j - length slicek = 0) as -> by lia.
-     rewrite <- app_comm_cons.
-     rewrite lookup_cons_eq_0.
-
-     iApply (imp_load with "Hl").
-     rewrite /continue; iIntros "!> Hl /=".
-     iApply imp_ret. encode. rewrite Hlookup. iSplit; first auto.
-     iCombine ("Hl Hslice2") as "Hslice2".
-     iPoseProof (big_sepL2_cons (λ _ l' x', pointsto l' dq (V #x')) with "Hslice2") as "Hslice2".
-     iPoseProof (big_sepL2_app with "Hslice1 Hslice2") as "Hslice".
-     iExists ls. iSplit; first (rewrite Hls; rewrite <- !app_assoc; auto). iSplit.
-     { iPureIntro. lia. }
-     rewrite {1}Hls.
-     rewrite Hj. rewrite drop_app drop_all Z.sub_diag drop_none. simpl.
-     assert (length xs = length (slicek ++ l :: slicerest)) as -> by lia.
-     rewrite take_app_length.
-     rewrite Hxs. rewrite Hlookup.
-     iApply "Hslice".
-   Qed.
-
 
 End array_reasoning.
